LambdaS5/coq/EjsSyntax.v
@@ -33,8 +33,8 @@ Inductive expr : Type :=
 | expr_if : expr -> expr -> expr -> expr
 | expr_set_field :  expr -> expr -> expr -> expr
 | expr_app : expr -> list expr -> expr
-| expr_func : option id -> list id -> prog -> expr
-| expr_func_stmt : id -> list id -> prog -> expr (* TODO find way to remove it *)
+| expr_func : option id -> list id -> prog -> string -> expr (* the string is program text *)
+| expr_func_stmt : id -> list id -> prog -> string -> expr (* TODO find way to remove it *)
 (* | expr_let : id -> expr -> expr -> expr *)
 | expr_fseq : expr -> expr -> expr
 | expr_seq : expr -> expr -> expr
